{"nbformat":4,"nbformat_minor":0,"metadata":{"colab":{"provenance":[],"collapsed_sections":["8ymhQNhO47PX","VgAmSDWuJjhE","u9hXb5nfKGsd","tiXRCA1BD92H","pC9MyJByEEFT","Ap7PBI0yFLsM","ExcSOA1f835V"],"authorship_tag":"ABX9TyPZbpWlnfIoN0IgVil9pNrD"},"kernelspec":{"name":"python3","display_name":"Python 3"},"language_info":{"name":"python"}},"cells":[{"cell_type":"markdown","source":["### Question"],"metadata":{"id":"8ymhQNhO47PX"}},{"cell_type":"markdown","source":["(Ex. 27, p. 36, Sec 1.1, Briggs) Find the inverse of\n","\n","$$\n","f(x) = \\sqrt{x + 2} \\quad \\text{for } x \\geq -2\n","$$"],"metadata":{"id":"mrCqIUJK49So"}},{"cell_type":"markdown","source":["#### Solution"],"metadata":{"id":"hikKexvZ5SuN"}},{"cell_type":"markdown","source":["\\begin{align}\n","x &= \\sqrt{y+2} \\\\\n","x^2 &= y + 2 \\\\\n","x^2 - 2 &= y \\\\\n","f^{-1}(x) &= x^2 - 2\n","\\end{align}"],"metadata":{"id":"7euiNP-E5Z4u"}},{"cell_type":"markdown","source":["##### Remark"],"metadata":{"id":"Ol0aZAfryaBa"}},{"cell_type":"markdown","source":["$$\n","f(x) = 2^x \\\\\n","f^{-1}(x) = \\log_2(x) \\\\\n","f(3) = 8 \\\\\n","f^{-1}(8) = 3 \\\\\n","f^{-1}(f(x)) = x \\\\\n","\\log_2(2^3) = 3\n","$$"],"metadata":{"id":"TWpsFT9-xQao"}},{"cell_type":"markdown","source":["### Question"],"metadata":{"id":"VgAmSDWuJjhE"}},{"cell_type":"markdown","source":["(Ex. 28, p. 36, Sec 1.3, Briggs) Find the inverse of\n","\n","\\begin{align}\n","f(x) = \\frac{2}{x^2 + 1} \\quad \\text{for } x \\geq 0\n","\\end{align}\n"],"metadata":{"id":"Z_fAeO22Jl59"}},{"cell_type":"markdown","source":["#### Solution"],"metadata":{"id":"u9hXb5nfKGsd"}},{"cell_type":"markdown","source":["Switching $x$ and $y$, $x = \\frac{2}{y^2 + 1}$. It follows $|y| = \\sqrt{\\frac{2}{x} - 1}$. Since domain of $f$ is $[0, \\infty)$, It is also the range of $f^{-1}$. So $|y| = y$."],"metadata":{"id":"VbMYHumBKKGY"}},{"cell_type":"markdown","source":["\\begin{align}\n","x &= \\frac{2}{y^2 + 1} \\\\\n","2 &= x(y^2 + 1) \\\\\n","2 &= xy^2 + x \\\\\n","2 - x &= xy^2 \\\\\n","\\frac{2}{x} - 1 &= y^2 \\\\\n","\\sqrt{ \\frac{2}{x} - 1 } &= \\sqrt{y^2} \\\\\n","&= \\pm y \\\\\n","&= y\n","\\end{align}"],"metadata":{"id":"SYrom6Y7P-0z"}},{"cell_type":"markdown","source":["$$\n","y = 3 \\\\\n","|y| = y = 3 \\\\\n","y = -3 \\\\\n","|y| = -y = -(-3) = 3 \\\\\n","|y| \\neq y\n","$$"],"metadata":{"id":"t6KIXl1YRpLn"}}]}