{"nbformat":4,"nbformat_minor":0,"metadata":{"colab":{"provenance":[],"collapsed_sections":["5heU9vV2lUZS","jT_pkGvHjPyL","2vyTgboclW8T","Ju_96fNKmlST","GBs1hZc4oGUU","9C3EahQ9pCxB","2nqi2A6YqBho","TKxD6JlEsHyq","yl42ktNCMb20","RpoK7gH1Qy61","Tz9qAeax5xE0","XpvBwRERflx2"],"authorship_tag":"ABX9TyOXHjeVEPCMjDctvud18/cO"},"kernelspec":{"name":"python3","display_name":"Python 3"},"language_info":{"name":"python"}},"cells":[{"cell_type":"markdown","source":["### Question"],"metadata":{"id":"5heU9vV2lUZS"}},{"cell_type":"markdown","source":["(ex. 11 (b), p. 31, sec. 1.3, Kolman) Compute $BA$ where\n","\\begin{align}\n","A = \\begin{bmatrix}\n","1 & 2 & 3 \\\\\n","2 & 1 & 4\n","\\end{bmatrix}\n","\\quad\n","B =\n","\\begin{bmatrix}\n","1 & 0  \\\\\n","2 & 1 \\\\\n","3 & 2\n","\\end{bmatrix}\n","\\end{align}"],"metadata":{"id":"0HaFFQSxjBKf"}},{"cell_type":"markdown","source":["#### Solution"],"metadata":{"id":"jT_pkGvHjPyL"}},{"cell_type":"markdown","source":["\\begin{align}\n","BA &= \\begin{bmatrix}\n","1 \\cdot 1 + 0 \\cdot 2 & 1 \\cdot 2 + 0 \\cdot 1 & 1 \\cdot 3 + 0 \\cdot 4 \\\\\n","2 \\cdot 1 + 1 \\cdot 2 & 2 \\cdot 2 + 1 \\cdot 1 & 2 \\cdot 3 + 1 \\cdot 4 \\\\\n","3 \\cdot 1 + 2 \\cdot 2 & 3 \\cdot 2 + 2 \\cdot 1 & 3 \\cdot 3 + 2 \\cdot 4\n","\\end{bmatrix} \\\\\n","&= \\begin{bmatrix}\n","1 & 2 & 3 \\\\\n","4 & 5 & 10 \\\\\n","7 & 8 & 17\n","\\end{bmatrix}\n","\\end{align}"],"metadata":{"id":"INO2jZ5-jRfx"}},{"cell_type":"markdown","source":["### Question"],"metadata":{"id":"2vyTgboclW8T"}},{"cell_type":"markdown","source":["(ex. 1 (b), p. 113, sec. 2.2, Kolman) Solve the following linear system using _Gaussian Elimination_.\n","\n","Note. _reduced row echelon form_ satisfies conditions (a), (b), (c), and (d). _Echelon form_ satisfies (a), (b), and (c).\n","\n","\\begin{align}\n","\\left [\n","\\begin{array}{cccc|c}\n","        1 & -3 & 4 & 1 & 0 \\\\\n","        0 & 0 & 1 & -1 & 4 \\\\\n","        0 & 0 & 0 & 1 & 1\n","\\end{array}\n","\\right ]\n","\\end{align}"],"metadata":{"id":"4i9Z-tynmS3z"}},{"cell_type":"markdown","source":["#### Solution"],"metadata":{"id":"Ju_96fNKmlST"}},{"cell_type":"markdown","source":["The system is already in echelon form.\n","\n","\\begin{align}\n","x - 3y + 4z + w &= 0 \\\\\n","z - w &= 4 \\\\\n","w &= 1\n","\\end{align}\n","\n","\\begin{align}\n","w &= 1 \\\\\n","z &= 5 \\\\\n","x &= 3y - 21\n","\\end{align}\n","\n","Solution is\n","\\begin{align}\n","\\begin{bmatrix} x \\\\ y \\\\ z \\\\ w \\end{bmatrix}\n","=\n","\\begin{bmatrix}\n","3y - 21 \\\\ y \\\\ 5 \\\\ 1\n","\\end{bmatrix}\n","\\end{align}\n","Where $y$ is a free-variable and $x$ is dependent on it."],"metadata":{"id":"wwrtAXqtmnIV"}},{"cell_type":"markdown","source":["### Question"],"metadata":{"id":"GBs1hZc4oGUU"}},{"cell_type":"markdown","source":["(ex. 12 (b), sec. 3.1, p. 145, kolman) Compute by the permutations method\n","\n","\\begin{align}\n","det \\begin{bmatrix}\n","2 & 4 & 5 \\\\\n","0 & -6 & 2 \\\\\n","0 & 0 & 3\n","\\end{bmatrix}\n","\\end{align}"],"metadata":{"id":"tgXUZgwuomxq"}},{"cell_type":"markdown","source":["#### Solution"],"metadata":{"id":"9C3EahQ9pCxB"}},{"cell_type":"markdown","source":["$(2)(-6)(3) + (4)(2)(0) + (5)(0)(0) - (5)(-6)(0) - (4)(0)(3) - (2)(2)(0) = -36$"],"metadata":{"id":"GzRqMeXzpFNO"}},{"cell_type":"markdown","source":["### Question"],"metadata":{"id":"2nqi2A6YqBho"}},{"cell_type":"markdown","source":["(ex. 3, p. 164, sec. 3.3, Kolman) Find the determinant by cofactor method of\n","\n","\\begin{bmatrix}\n","-1 & 2 & 3 \\\\\n","-2 & 5 & 4 \\\\\n","0 & 1 & -3\n","\\end{bmatrix}"],"metadata":{"id":"gt6ZYV2cqDKf"}},{"cell_type":"markdown","source":["#### Solution"],"metadata":{"id":"TKxD6JlEsHyq"}},{"cell_type":"markdown","source":["On the third row:\n","\\begin{align}\n","&(-1)^4 (0)\n","\\begin{vmatrix}\n","2 & 3 \\\\\n","5 & 4\n","\\end{vmatrix}\n","+\n","(-1)^5 (1)\n","\\begin{vmatrix}\n","-1 & 3 \\\\\n","-2 & 4\n","\\end{vmatrix}\n","+\n","(-1)^6 (-3)\n","\\begin{vmatrix}\n","-1 & 2 \\\\\n","-2 & 5\n","\\end{vmatrix} \\\\\n","&= 0 - (-4 - (-6)) + (-3)(-5 - (-4)) \\\\\n","&= -2 + 3 = 1\n","\\end{align}"],"metadata":{"id":"XXp1iR4tqWVB"}},{"cell_type":"markdown","source":["### Question"],"metadata":{"id":"yl42ktNCMb20"}},{"cell_type":"markdown","source":["(ex. 2, p. 164, sec. 3.5, Kolman) Solve the following system using _Cramer_.\n","\n","\\begin{align}\n","\\begin{bmatrix}\n","1 & 1 & 1 & -2 \\\\\n","0 & 2 & 1 & 3 \\\\\n","2 & 1 & -1 & 2 \\\\\n","1 & -1 & 0 & 1\n","\\end{bmatrix}\n","\\begin{bmatrix}\n","x_1 \\\\ x_2 \\\\ x_3 \\\\ x_4\n","\\end{bmatrix}\n","=\n","\\begin{bmatrix}\n","-4 \\\\ 4 \\\\ 5 \\\\ 4\n","\\end{bmatrix}\n","\\end{align}\n","Given\n","\\begin{align}\n","\\det A &= \\det\n","\\begin{bmatrix}\n","1 & 1 & 1 & -2 \\\\\n","0 & 2 & 1 & 3 \\\\\n","2 & 1 & -1 & 2 \\\\\n","1 & -1 & 0 & 1\n","\\end{bmatrix}\n","= 26 \\\\ \\\\\n","\\det A_1 &= \\det\n","\\begin{bmatrix}\n","-4 & 1 & 1 & -2 \\\\\n","4 & 2 & 1 & 3 \\\\\n","5 & 1 & -1 & 2 \\\\\n","4 & -1 & 0 & 1\n","\\end{bmatrix}\n","= -52 \\\\\n","\\det A_2 &= \\det\n","\\begin{bmatrix}\n","1 & -4 & 1 & -2 \\\\\n","0 & 4 & 1 & 3 \\\\\n","2 & 5 & -1 & 2 \\\\\n","1 & 4 & 0 & 1\n","\\end{bmatrix}\n","= 0 \\\\ \\\\\n","\\det A_3 &= \\det\n","\\begin{bmatrix}\n","1 & 1 & -4 & -2 \\\\\n","0 & 2 & 4 & 3 \\\\\n","2 & 1 & 5 & 2 \\\\\n","1 & -1 & 4 & 1\n","\\end{bmatrix}\n","= 26 \\\\ \\\\\n","\\det A_4 &= \\det\n","\\begin{bmatrix}\n","1 & 1 & 1 & -4 \\\\\n","0 & 2 & 1 & 4 \\\\\n","2 & 1 & -1 & 5 \\\\\n","1 & -1 & 0 & 4\n","\\end{bmatrix}\n","= 26\n","\\end{align}"],"metadata":{"id":"klBo7PNKLaof"}},{"cell_type":"markdown","source":["#### Solution"],"metadata":{"id":"RpoK7gH1Qy61"}},{"cell_type":"markdown","source":["\\begin{align}\n","x_1 &= \\frac{det \\, A_1}{det \\, A} = \\frac{-30}{-30} = 1 \\\\\n","x_2 &= \\frac{det \\, A_2}{det \\, A} = \\frac{30}{-30} = -1 \\\\\n","x_3 &= \\frac{det \\, A_3}{det \\, A} = \\frac{0}{-30} = 0 \\\\\n","x_4 &= \\frac{det \\, A_4}{det \\, A} = \\frac{-60}{-30} = 2\n","\\end{align}"],"metadata":{"id":"1XibbZhoNU0y"}},{"cell_type":"markdown","source":["### Question"],"metadata":{"id":"Tz9qAeax5xE0"}},{"cell_type":"markdown","source":["(ex. 4, p. 169, sec. 3.4, Kolman) Find the inverse using the adjoint matrix method.\n","\n","\\begin{bmatrix}\n","2 & 1 & 3 \\\\\n","-1 & 2 & 0 \\\\\n","3 & -2 & 1\n","\\end{bmatrix}"],"metadata":{"id":"nYOycXPf6Fur"}},{"cell_type":"markdown","source":["#### Solution"],"metadata":{"id":"XpvBwRERflx2"}},{"cell_type":"markdown","source":["Minors.\n","\n","\\begin{align}\n","det(M_{11}) &= \\begin{vmatrix} 2 & 0 \\\\ -2 & 1 \\end{vmatrix} = 2 - 0 = 2 \\\\\n","det(M_{12}) &= \\begin{vmatrix} -1 & 0 \\\\ 3 & 1 \\end{vmatrix} = -1 - 0 = -1 \\\\\n","det(M_{13}) &= \\begin{vmatrix} -1 & 2 \\\\ 3 & -2 \\end{vmatrix} = 2 - 6 = -4 \\\\\n","det(M_{21}) &= \\begin{vmatrix} 1 & 3 \\\\ -2 & 1 \\end{vmatrix} = 1 - (-6) = 7 \\\\\n","det(M_{22}) &= \\begin{vmatrix} 2 & 3 \\\\ 3 & 1 \\end{vmatrix} = 2 - 9 = -7 \\\\\n","det(M_{23}) &= \\begin{vmatrix} 2 & 1 \\\\ 3 & -2 \\end{vmatrix} = -4 - 3 = -7 \\\\\n","det(M_{31}) &= \\begin{vmatrix} 1 & 3 \\\\ 2 & 0 \\end{vmatrix} = 0 - 6 = -6 \\\\\n","det(M_{32}) &= \\begin{vmatrix} 2 & 3 \\\\ -1 & 0 \\end{vmatrix} = 0 - (-3) = 3 \\\\\n","det(M_{33}) &= \\begin{vmatrix} 2 & 1 \\\\ -1 & 2 \\end{vmatrix} = 4 - (-1) = 5 \\\\\n","\\end{align}\n","\n","Cofactors\n","\n","\\begin{align}\n","A_{11} = (-1)^{1+1} det(M_{11}) = 1 \\cdot 2 = 2 \\\\\n","A_{12} = (-1)^{1+2} det(M_{12}) = -1 \\cdot -1 = 1 \\\\\n","A_{13} = (-1)^{1+3} det(M_{13}) = 1 \\cdot -4 = -4 \\\\\n","A_{21} = (-1)^{2+1} det(M_{21}) = -1 \\cdot 7 = -7 \\\\\n","A_{22} = (-1)^{2+2} det(M_{22}) = 1 \\cdot -7 = -7 \\\\\n","A_{23} = (-1)^{2+3} det(M_{23}) = -1 \\cdot -7 = 7 \\\\\n","A_{31} = (-1)^{3+1} det(M_{31}) = 1 \\cdot -6 = -6 \\\\\n","A_{32} = (-1)^{3+2} det(M_{32}) = -1 \\cdot 3 = -3 \\\\\n","A_{33} = (-1)^{3+3} det(M_{33}) = 1 \\cdot 5 = 5\n","\\end{align}\n","\n","Determinant\n","\n","$$a_{13} A_{13} + a_{23} A_{23} + a_{33} A_{33} = (3 \\cdot -4 )+ 0 + (1 \\cdot 5) = -7$$\n","\n","Adjoint Matrix\n","\n","$$\n","adj \\, A =\n","\\begin{bmatrix}\n","2 & -7 & -6 \\\\\n","1 & -7 & -3 \\\\\n","-4 & 7 & 5\n","\\end{bmatrix}\n","$$\n","\n","Inverse Matrix\n","\n","$$\n","A^{-1} = \\frac{1}{det \\, A} \\cdot adj \\, A =\n","\\begin{bmatrix}\n","\\frac{-2}{7} & 1 & \\frac{6}{7} \\\\\n","\\frac{-1}{7} & 1 &  \\frac{3}{7} \\\\\n","\\frac{-4}{7} & -1 & \\frac{-5}{7}\n","\\end{bmatrix}\n","$$"],"metadata":{"id":"WVWqk6Vo_Y0C"}}]}