{"nbformat":4,"nbformat_minor":0,"metadata":{"colab":{"provenance":[],"collapsed_sections":["577haIZN7Nb8","8epwp5Pd7l3-","0AT4dY1I-XEF","3OchRo75--1U","Fye9CrysAzs-","ZhGrkxUsBNOJ","ZEZ2Mba8x8XA","U_n0-1Zjyd5C","yEqHreYux4F2"],"authorship_tag":"ABX9TyMwucWl1mXlSOHcqjV7TTxm"},"kernelspec":{"name":"python3","display_name":"Python 3"},"language_info":{"name":"python"}},"cells":[{"cell_type":"markdown","source":["### Question"],"metadata":{"id":"577haIZN7Nb8"}},{"cell_type":"markdown","source":["(ex. 7, p. 124, sec. 2.3, Kolman) Find the inverse of by the procedure of page 121\n","\n","$$\n","A =\n","\\begin{bmatrix} 1 & 3 \\\\ 2 & 4 \\end{bmatrix}\n","$$"],"metadata":{"id":"GtrVIOvK7Oqw"}},{"cell_type":"markdown","source":["#### Solution"],"metadata":{"id":"8epwp5Pd7l3-"}},{"cell_type":"markdown","source":["\\begin{align}\n","\\left [\n","A \\, \\bigg | \\, I_2\n","\\right ]\n","&=\n","\\left [\n","\\begin{array}{cc|cc}\n","        1 & 3 & 1 & 0 \\\\\n","        2 & 4 & 0 & 1 \\\\\n","    \\end{array}\n","\\right ] \\\\\n","&\\rightarrow^{R_2 = -2 R_1 + R_2}\n","\\left [\n","\\begin{array}{cc|cc}\n","        1 & 3 & 1 & 0 \\\\\n","        0 & -2 & -2 & 1 \\\\\n","    \\end{array}\n","\\right ] \\\\\n","&\\rightarrow^{R_2 = (1/-2) R_2}\n","\\left [\n","\\begin{array}{cc|cc}\n","        1 & 3 & 1 & 0 \\\\\n","        0 & 1 & 1 & \\frac{-1}{2} \\\\\n","    \\end{array}\n","\\right ] \\\\\n","&\\rightarrow^{R_1 = -3 R_2 + R_1}\n","\\left [\n","\\begin{array}{cc|cc}\n","        1 & 0 & -2 & \\frac{3}{2} \\\\\n","        0 & 1 & 1 & \\frac{-1}{2} \\\\\n","    \\end{array}\n","\\right ] \\\\\n","&=\n","\\left [\n","I_2 \\, \\bigg | \\, A^{-1}\n","\\right ]\n","\\end{align}"],"metadata":{"id":"zinFfOI07pDr"}},{"cell_type":"markdown","source":["### Question"],"metadata":{"id":"0AT4dY1I-XEF"}},{"cell_type":"markdown","source":["Given\n","\n","\\begin{align}\n","A = \\begin{bmatrix} 1 & 3 \\\\ 2 & 4 \\end{bmatrix} \\quad\n","A^{-1} = \\begin{bmatrix} -2 & \\frac{3}{2} \\\\ 1 & \\frac{-1}{2} \\end{bmatrix} \\quad\n","B = \\begin{bmatrix} 7 \\\\ 7 \\end{bmatrix}\n","\\end{align}\n","\n","What is the solution of the system\n","$$\n","AX = B\n","$$"],"metadata":{"id":"BTWETlM9-ZD9"}},{"cell_type":"markdown","source":["#### Solution"],"metadata":{"id":"3OchRo75--1U"}},{"cell_type":"markdown","source":["\\begin{align}\n","AX &= B \\\\\n","A^{-1} AX &= A^{-1} B \\\\\n","I_2 X &= A^{-1} B \\\\\n","X &= \\begin{bmatrix} -14 + \\frac{21}{2} \\\\ 7 + \\frac{-7}{2} \\end{bmatrix} = \\begin{bmatrix} \\frac{-7}{2} \\\\ \\frac{7}{2} \\end{bmatrix}\n","\\end{align}"],"metadata":{"id":"rf7dfiTH_Bh4"}},{"cell_type":"markdown","source":["### Question"],"metadata":{"id":"Fye9CrysAzs-"}},{"cell_type":"markdown","source":["(ex. 9, p. 124, sec. 2.3, Kolman) Is the following matrix singular?\n","\n","$$\n","\\begin{bmatrix}\n","1 & 3 \\\\\n","2 & 6\n","\\end{bmatrix}\n","$$"],"metadata":{"id":"a1h0lBeuA1fn"}},{"cell_type":"markdown","source":["#### Solution"],"metadata":{"id":"ZhGrkxUsBNOJ"}},{"cell_type":"markdown","source":["Yes it is singular, i.e non-invertible, Since its determinant is\n","$$\n","1 \\cdot 6 - 3 \\cdot 2 = 6 - 6 = 0\n","$$"],"metadata":{"id":"OpkM7mCTBO6E"}},{"cell_type":"markdown","source":["### Question"],"metadata":{"id":"ZEZ2Mba8x8XA"}},{"cell_type":"markdown","source":["(ex. 2 (c), p. 155, sec. 3.2, Kolman) Compute the determinant using properties of determinants.\n","\n","$$\n","A =\n","\\begin{bmatrix}\n","3 & 4 & 2 \\\\\n","2 & 5 & 0 \\\\\n","3 & 0 & 0\n","\\end{bmatrix}\n","$$"],"metadata":{"id":"9ekP4SHMx97D"}},{"cell_type":"markdown","source":["#### Solution"],"metadata":{"id":"U_n0-1Zjyd5C"}},{"cell_type":"markdown","source":["Consider the matrix obtained by interchanging first and third rows\n","\n","$$\n","A_{R_1 \\leftrightarrow R_3} =\n","\\begin{bmatrix}\n","3 & 0 & 0 \\\\\n","2 & 5 & 0 \\\\\n","3 & 4 & 2\n","\\end{bmatrix}\n","$$\n","\n","From theorem 3.7 (page 149), Its determinant is the multiplication of diagonal entries.\n","\n","$$\n","2 \\cdot 5 \\cdot 3 = 30\n","$$\n","\n","From theorem 3.2 (page 147), $\\det A = - \\det A_{R_1 \\leftrightarrow R_3} = -30$."],"metadata":{"id":"jmT--R-myhOf"}},{"cell_type":"markdown","source":["### Question"],"metadata":{"id":"yEqHreYux4F2"}},{"cell_type":"markdown","source":["(ex. 7 (b), p. 169, sec. 3.4, Kolman)  Find the inverse if it exists using the adjoint matrix method.\n","\n","\\begin{align}\n","A =\n","\\begin{bmatrix}\n","4 & 2 & 2 \\\\\n","0 & 1 & 2 \\\\\n","1 & 0 & 3\n","\\end{bmatrix}\n","\\end{align}"],"metadata":{"id":"Wizzlvj2ebRs"}},{"cell_type":"markdown","source":["#### Solution"],"metadata":{"id":"ay7LgbMcujy5"}},{"cell_type":"markdown","source":["Minors\n","\\begin{align}\n","\\det M_{11} &= \\begin{vmatrix} 1 & 2 \\\\ 0 & 3 \\end{vmatrix} = (3) - (0) = 3 \\\\\n","\\det M_{12} &= \\begin{vmatrix} 0 & 2 \\\\ 1 & 3 \\end{vmatrix} = (0) - (2) = -2 \\\\\n","\\det M_{13} &= \\begin{vmatrix} 0 & 1 \\\\ 1 & 0 \\end{vmatrix} = (0) - (1) = -1 \\\\\n","\\det M_{21} &= \\begin{vmatrix} 2 & 2 \\\\ 0 & 3 \\end{vmatrix} = (6) - (0) = 6 \\\\\n","\\det M_{22} &= \\begin{vmatrix} 4 & 2 \\\\ 1 & 3 \\end{vmatrix} = (12) - (2) = 10 \\\\\n","\\det M_{23} &= \\begin{vmatrix} 4 & 2 \\\\ 1 & 0 \\end{vmatrix} = (0) - (2) = -2 \\\\\n","\\det M_{31} &= \\begin{vmatrix} 2 & 2 \\\\ 1 & 2 \\end{vmatrix} = (4) - (2) = 2 \\\\\n","\\det M_{32} &= \\begin{vmatrix} 4 & 2 \\\\ 0 & 2 \\end{vmatrix} = (8) - (0) = 8 \\\\\n","\\det M_{33} &= \\begin{vmatrix} 4 & 2 \\\\ 0 & 1 \\end{vmatrix} = (4) - (0) = 4 \\\\\n","\\end{align}\n","\n","Cofactors\n","\\begin{align}\n","A_{11} &= (-1)^{1+1} \\det M_{11} = 3 \\\\\n","A_{12} &= (-1)^{1+2} \\det M_{12} = 2 \\\\\n","A_{13} &= (-1)^{1+3} \\det M_{13} = -1 \\\\\n","A_{21} &= (-1)^{2+1} \\det M_{21} = -6 \\\\\n","A_{22} &= (-1)^{2+2} \\det M_{22} = 10 \\\\\n","A_{23} &= (-1)^{2+3} \\det M_{23} = 2 \\\\\n","A_{31} &= (-1)^{3+1} \\det M_{31} = 2 \\\\\n","A_{32} &= (-1)^{3+2} \\det M_{32} = -8 \\\\\n","A_{33} &= (-1)^{3+3} \\det M_{33} = 4 \\\\\n","\\end{align}\n","\n","Determinant (first column)\n","$$\n","a_{11} A_{11} + a_{21} A_{21} + a_{31} A_{31} = 4 (3) + 0 + 1 (2) = 12 + 2 = 14\n","$$\n","\n","Adjoint Matrix\n","\n","$$\n","adj \\, M =\n","\\begin{bmatrix}\n","3 & -6 & 2 \\\\\n","2 & 10 & -8 \\\\\n","-1 & 2 & 4\n","\\end{bmatrix}\n","$$\n","\n","Inverse Matrix\n","$$\n","M^{-1} = \\frac{1}{\\det M} \\cdot adj \\, M =\n","\\begin{bmatrix}\n","\\frac{3}{14} & \\frac{-3}{7} & \\frac{1}{7} \\\\\n","\\frac{1}{7} & \\frac{5}{7} & \\frac{-4}{7} \\\\\n","\\frac{-1}{14} & \\frac{1}{7} & \\frac{2}{7}\n","\\end{bmatrix}\n","$$"],"metadata":{"id":"aepvGOxJu4D7"}}]}