{"nbformat":4,"nbformat_minor":0,"metadata":{"colab":{"provenance":[],"collapsed_sections":["tgOl6de6l_e6","f2vsvUw-wLeY","hBGNf99LmbQB","g0MNNDzDqi1d","qHUapLHz2qcW","rt-bOMq7ybRf"],"authorship_tag":"ABX9TyNy1sgOca+haqVQuGnJOzRe"},"kernelspec":{"name":"python3","display_name":"Python 3"},"language_info":{"name":"python"}},"cells":[{"cell_type":"markdown","source":["### Question"],"metadata":{"id":"tgOl6de6l_e6"}},{"cell_type":"markdown","source":["(ex. 26, p. 513, sec. 7.2, Briggs) Evaluate\n","\n","$$\n","A = \\int x^2 \\ln^2 x \\, dx\n","$$"],"metadata":{"id":"VJcfnJ0jmCqA"}},{"cell_type":"markdown","source":["#### Hints"],"metadata":{"id":"f2vsvUw-wLeY"}},{"cell_type":"markdown","source":["- You will use substitution by parts twice\n","- Set $u = ln^2 x$"],"metadata":{"id":"urVbr7_JwNQG"}},{"cell_type":"markdown","source":["#### Solution"],"metadata":{"id":"hBGNf99LmbQB"}},{"cell_type":"markdown","source":["\\begin{align}\n","u &= \\ln^2 x \\quad du = 2 \\frac{1}{x} \\ln(x) \\, dx \\\\\n","dv &= x^2 \\, dx \\quad v = \\frac{1}{3} x^3\n","\\end{align}\n","\n","\\begin{align}\n","A &= \\frac{1}{3} x^3 \\ln^2 x - \\int \\frac{1}{3} x^3 2 \\frac{1}{x} \\ln(x) \\, dx \\\\\n","&= \\frac{1}{3} x^3 \\ln^2 x - \\frac{2}{3} \\int x^2 ln(x) \\, dx\n","\\end{align}\n","\n","We now evaluate\n","$$\n","A' = \\int x^2 ln(x) \\, dx\n","$$\n","\n","\\begin{align}\n","u &= \\ln x \\quad du = \\frac{1}{x} \\, dx \\\\\n","dv &= x^2 \\, dx \\quad v = \\frac{1}{3} x^3\n","\\end{align}\n","\n","\\begin{align}\n","A' &= \\frac{1}{3} x^3 \\ln(x) - \\int \\frac{1}{3} x^3 \\frac{1}{x} \\, dx \\\\\n","&= \\frac{1}{3} x^3 \\ln(x) - \\frac{1}{3} \\int x^2 \\frac{1}{x} \\, dx \\\\\n","&= \\frac{1}{3} x^3 \\ln(x) - \\frac{1}{3} \\frac{1}{3} x^3 \\\\\n","&= \\frac{1}{9} x^3 (3 \\ln(x) - 1) + C\n","\\end{align}\n","\n","It follows\n","\\begin{align}\n","A &= \\frac{1}{3} x^3 \\ln^2(x) - \\frac{2}{3} \\cdot \\frac{1}{9} x^3 (3\\ln(x) - 1) \\\\\n","&= \\frac{x^3}{27} (9 \\ln^2 x - 6 \\ln x + 2) + C\n","\\end{align}"],"metadata":{"id":"OWQqJWu7mc9_"}},{"cell_type":"markdown","source":["### Question"],"metadata":{"id":"g0MNNDzDqi1d"}},{"cell_type":"markdown","source":["(ex. 36, p. 513, sec. 7.2, Briggs) Evaluate\n","\n","$$\n","A = \\int_0^{\\frac{1}{\\sqrt{2}}} x \\tan^{-1}(x^2) \\, dx\n","$$\n"],"metadata":{"id":"BuHUH5p-ql-v"}},{"cell_type":"markdown","source":["#### Hints"],"metadata":{"id":"qHUapLHz2qcW"}},{"cell_type":"markdown","source":["- You will integrate twice, the second one by substitution.\n","- Recall $[ tan^{-1}(x) ]' = \\frac{1}{1+x^2}$, p. 213 in Briggs.\n","- Set $u(x) = \\tan^{-1}(x^2)$."],"metadata":{"id":"ur8g1q-u2a_y"}},{"cell_type":"markdown","source":["#### Solution"],"metadata":{"id":"rt-bOMq7ybRf"}},{"cell_type":"markdown","source":["\\begin{align}\n","u(x) &= \\tan^{-1}(x^2) \\quad u'(x) = \\frac{2x}{1 + x^4} \\, dx \\\\\n","v'(x) &= x \\, dx \\quad v(x) = \\frac{1}{2} x^2\n","\\end{align}\n","\n","\\begin{align}\n","A = tan^{-1}(x^2) \\cdot \\frac{1}{2} x^2 \\bigg |_0^{1/\\sqrt{2}} - \\int_0^{1/\\sqrt{2}} \\frac{x^3}{1 + x^4} \\, dx\n","\\end{align}\n","\n","We now evaluate by substitution\n","$$\n","A' = \\int_0^{1/\\sqrt{2}} \\frac{x^3}{1 + x^4} \\, dx\n","$$\n","\n","$$\n","u = 1 + x^4 \\quad du = 4x^3 \\, dx\n","$$\n","\n","\\begin{align}\n","A' &= \\frac{1}{4} \\int_1^{5/4} \\frac{1}{u} \\, du \\\\\n","&= \\frac{1}{4} \\ln(u) \\bigg |_1^{5/4} \\\\\n","&= \\frac{1}{4} (\\ln(5/4) - ln(1)) \\\\\n","&= \\frac{1}{4} \\ln(5/4)\n","\\end{align}\n","\n","It follows\n","\\begin{align}\n","A &= \\left [ tan^{-1}(1/2) \\frac{1}{2} \\frac{1}{2} - 0 \\right ] - \\frac{1}{4} \\ln(5/4) \\\\\n","&= \\frac{1}{4} \\left [ \\tan^{-1}(1/2) - \\ln(5/4) \\right ]\n","\\end{align}"],"metadata":{"id":"LznL7Jb5wY1E"}}]}