{"nbformat":4,"nbformat_minor":0,"metadata":{"colab":{"provenance":[],"collapsed_sections":["zNeLdMUPL5RJ","AACnAix49gwT","eI2jABdG-zOR"],"authorship_tag":"ABX9TyPw8ctld8wNr5IrE4+3c5Gn"},"kernelspec":{"name":"python3","display_name":"Python 3"},"language_info":{"name":"python"}},"cells":[{"cell_type":"markdown","source":["- Note the theorems in pages: 165, 518, 519, 525.\n","- Recall $sin^2 x + cos^2 x = 1$."],"metadata":{"id":"wcIUWdPtZXTu"}},{"cell_type":"markdown","source":["### Question"],"metadata":{"id":"zNeLdMUPL5RJ"}},{"cell_type":"markdown","source":["(ex. 7, p. 529, sec. 7.4, Briggs) Evaluate\n","$$\n","A = \\int_0^{5/2} \\frac{dx}{\\sqrt{25 - x^2}}\n","$$"],"metadata":{"id":"d8JA-5QEL6ky"}},{"cell_type":"markdown","source":["#### Solution"],"metadata":{"id":"6StJoPX8MNRu"}},{"cell_type":"markdown","source":["\\begin{align}\n","x &= 5 \\sin \\theta \\\\\n","dx &= 5 \\cos \\theta \\, d\\theta \\\\\n","\\sqrt{25 - x^2} &= \\sqrt{5^2 - x^2} = \\sqrt{5^2 - (5 \\sin \\theta)^2} = \\sqrt{5^2 (1 - \\sin^2 \\theta)} = \\sqrt{5^2 \\cos^2 \\theta} = 5 \\cos \\theta \\\\\n","\\frac{5}{2} = 5 \\sin \\theta &\\rightarrow \\theta = \\frac{\\pi}{6} \\\\\n","0 = 5 \\sin \\theta &\\rightarrow \\theta = 0 \\\\\n","A &= \\int_0^{\\pi/6} \\frac{5 \\cos \\theta}{5 \\cos \\theta} \\, d\\theta \\\\\n","&= \\int_0^{\\pi/6} d\\theta \\\\\n","&= \\theta \\bigg |_0^{\\pi/6} = \\frac{\\pi}{6} - 0 = \\frac{\\pi}{6}\n","\\end{align}"],"metadata":{"id":"MOTHuosDMO2q"}},{"cell_type":"markdown","source":["### Question"],"metadata":{"id":"AACnAix49gwT"}},{"cell_type":"markdown","source":["(ex. 13, p. 529, sec. 7.4, Briggs) Evaluate\n","$$\n","A = \\int \\frac{1}{(16-x^2)^{1/2}} \\, dx\n","$$"],"metadata":{"id":"wc_0pjBDSVxE"}},{"cell_type":"markdown","source":["#### Solution"],"metadata":{"id":"ll4rT1HJ9ifQ"}},{"cell_type":"markdown","source":["\\begin{align}\n","\\sqrt{16-x^2} &= \\sqrt{4^2-x^2} = \\sqrt{a^2-x^2} \\\\\n","a &= 4 \\\\\n","x &= a \\sin \\theta = 4 \\sin \\theta \\\\\n","dx &= 4 \\cos \\theta \\, d \\theta \\\\\n","\\sqrt{4^2 - x^2} &= \\sqrt{4^2 - (4 \\sin \\theta)^2} = \\sqrt{4^2 (1-sin^2 \\theta)} = \\sqrt{4^2 \\cos^2 \\theta} = 4 \\cos \\theta \\\\\n","A &= \\int \\frac{4 \\cos \\theta}{4 \\cos \\theta} \\, d \\theta \\\\\n","&= \\int 1 \\, d \\theta \\\\\n","&= \\theta + C \\\\\n","&= \\sin^{-1} \\left (\\frac{x}{4} \\right ) + C\n","\\end{align}"],"metadata":{"id":"MrB4jBqg9j2J"}},{"cell_type":"markdown","source":["### Question"],"metadata":{"id":"eI2jABdG-zOR"}},{"cell_type":"markdown","source":["(ex. 21, p. 529, sec. 7.4, Briggs) Evaluate\n","$$\n","\\int \\frac{1}{x^2 \\sqrt{x^2 + 9}} \\, dx\n","$$"],"metadata":{"id":"kCHZoB4MJStL"}},{"cell_type":"markdown","source":["#### Solution"],"metadata":{"id":"OMSZj2wOJnsr"}},{"cell_type":"markdown","source":["\\begin{align}\n","\\sqrt{9+x^2} &= \\sqrt{3^2+x^2} = \\sqrt{a^2 +x^2} \\\\\n","a &= 3 \\\\\n","x &= a \\tan \\theta = 3 \\tan \\theta \\\\\n","dx &= 3 \\sec^2 \\theta \\, d \\theta \\\\\n","\\sqrt{x^2 + 9} &= \\sqrt{(3 \\tan \\theta)^2 + 9} = \\sqrt{3^2 \\sec^2 \\theta} = |3 \\sec \\theta | = 3 \\sec \\theta \\\\\n","A &= \\int 3 \\sec^2 \\theta \\cdot \\frac{1}{3^2 \\tan^2 \\theta} \\cdot \\frac{1}{3 \\ sec \\theta} \\, d \\theta \\\\\n","&= \\int \\sec \\theta \\cdot \\frac{1}{3^2 \\tan^2 \\theta} \\, d \\theta \\\\\n","&= \\frac{1}{9} \\cdot \\int \\frac{1}{\\cos \\theta} \\cdot \\frac{\\cos^2 \\theta}{\\sin^2 \\theta} \\\\\n","&= \\frac{1}{9} \\cdot \\int \\cos \\theta \\cdot \\frac{1}{\\sin^2 \\theta} \\, d \\theta \\\\\n","u &= \\sin \\theta \\\\\n","du &= \\cos \\theta \\, d \\theta \\\\\n","A &= \\frac{1}{9} \\int \\frac{1}{u^2} \\, du \\\\\n","&= \\frac{1}{9} \\cdot -1 \\cdot u^{-1} \\\\\n","&= \\frac{-1}{9} \\cdot \\frac{1}{\\sin \\theta} \\\\\n","&= \\frac{-\\sqrt{x^2 + 9}}{9x}\n","\\end{align}"],"metadata":{"id":"1R2TuH9hJpob"}},{"cell_type":"markdown","source":["### Question"],"metadata":{"id":"EynWsFM5Nw7V"}},{"cell_type":"markdown","source":["(ex. 31, p. 529, sec. 7.4, Briggs) Evaluate\n","$$\n","\\int \\frac{\\sqrt{x^2 - 9}}{x} \\, dx \\quad x > 3\n","$$"],"metadata":{"id":"QFunCa_MNyxq"}},{"cell_type":"markdown","source":["#### Solution"],"metadata":{"id":"ad3i4HH8X4-M"}},{"cell_type":"markdown","source":["\\begin{align}\n","\\sqrt{x^2 - 9} &= \\sqrt{x^2 - 3^2} = \\sqrt{x^2 - a^2} \\\\\n","a &= 3 \\\\\n","x &= 3 \\sec \\theta \\\\\n","dx &= 3 \\sec \\theta \\tan \\theta \\\\\n","A &= \\int 3 \\tan \\theta \\cdot \\frac{1}{3 \\sec \\theta} \\cdot 3 \\sec \\theta \\, d \\theta \\\\\n","&= 3 \\int \\tan^2 \\theta \\, d \\theta \\\\\n","&= 3 \\cdot  \\left (\\frac{\\tan \\theta}{1} - \\theta \\right ) + C \\\\\n","&= 3 \\cdot \\left [ \\frac{\\sqrt{x^2 - 3^2}}{3} - sec^{-1}(x/3) \\right ] + C \\\\\n","&= \\sqrt{x^2 - 9} - 3 \\sec^{-1}(x/3) + C\n","\\end{align}"],"metadata":{"id":"Ixv2YnRUX7ud"}}]}