{"nbformat":4,"nbformat_minor":0,"metadata":{"colab":{"provenance":[],"collapsed_sections":["NgXTdVgrClWu","TUcGsbW0CcKN","yY8CGZ55yUNK"],"authorship_tag":"ABX9TyP+3ILcOEw2DoL8Wi+ok5v0"},"kernelspec":{"name":"python3","display_name":"Python 3"},"language_info":{"name":"python"}},"cells":[{"cell_type":"markdown","source":["### Question"],"metadata":{"id":"_gV4mz5lAkBW"}},{"cell_type":"markdown","source":["(ex. 45, sec. 5.5, p. 383, Briggs) Evaluate\n","\n","$$\n","A = \\int_{\\pi/4}^{\\pi/2} \\frac{\\cos x}{\\sin^2 x} \\, dx\n","$$"],"metadata":{"id":"4mqHXwdd6qAH"}},{"cell_type":"markdown","source":["#### Solution"],"metadata":{"id":"NgXTdVgrClWu"}},{"cell_type":"markdown","source":["Set\n","\\begin{align}\n","u &= \\sin x \\\\\n","du &= \\cos x \\, dx\n","\\end{align}\n","Note\n","\\begin{align}\n","u(\\frac{\\pi}{2}) &= \\sin(\\frac{\\pi}{2}) = 1 \\\\\n","u(\\frac{\\pi}{4}) &= \\sin(\\frac{\\pi}{4}) = \\frac{\\sqrt{2}}{2}\n","\\end{align}\n","Then\n","\\begin{align}\n","A &= \\int_{ \\frac{\\sqrt{2}}{2} }^1 \\frac{1}{u^2} \\, du \\\\\n","&= -1 \\cdot u^{-1} \\bigg |_{\\frac{\\sqrt{2}}{2}}^{1} \\\\\n","&= -1 \\cdot (1)^{-1} - \\left (- \\left (\\frac{\\sqrt{2}}{2} \\right )^{-1} \\right ) \\\\\n","&= -1 + \\frac{2}{\\sqrt{2}} \\\\\n","&= \\sqrt{2} - 1\n","\\end{align}"],"metadata":{"id":"yzhpN7HoCn8T"}},{"cell_type":"markdown","source":["### Question"],"metadata":{"id":"TUcGsbW0CcKN"}},{"cell_type":"markdown","source":["(ex. 52, sec. 5.5, p. 383, Briggs) Evaluate\n","\\begin{align}\n","A = \\int_0^{\\ln 4} \\frac{e^x}{3 + 2e^x} dx\n","\\end{align}"],"metadata":{"id":"rqIOk7Ckpycn"}},{"cell_type":"markdown","source":["#### Hint"],"metadata":{"id":"yY8CGZ55yUNK"}},{"cell_type":"markdown","source":["- (Abstract; Pattern) Decompose the algebraic expressions. Imagine one of them the derivative of the other.\n","- Multiply by $\\frac{2}{2}$.\n","- Recall $[e^x]' = e^x$."],"metadata":{"id":"mS4T3fQ1yWzY"}},{"cell_type":"markdown","source":["#### Solution"],"metadata":{"id":"5aTrY6wcySq9"}},{"cell_type":"markdown","source":["\\begin{align}\n","A &= \\frac{1}{2} \\int_0^{\\ln 4} \\frac{2e^x}{3 + 2e^x} dx \\\\\n","g(x) &= 3 + 2e^x \\\\\n","g'(x) &= 2e^x \\\\\n","f(x) &= \\frac{1}{x} \\\\\n","A &= \\frac{1}{2} \\int_0^{\\ln 4} f(g(x)) \\cdot g'(x) \\\\\n","&= \\frac{1}{2} \\int_{g(0)}^{g(\\ln 4)} f(u) \\, du \\\\\n","&= \\frac{1}{2} \\int_5^{11} \\frac{1}{u} \\, du \\\\\n","&= \\frac{1}{2} \\cdot \\ln u \\bigg |_5^{11} \\\\\n","&= \\frac{1}{2} \\cdot \\ln 11 - \\ln 5 \\\\\n","&= \\frac{\\ln(11/5)}{2}\n","\\end{align}"],"metadata":{"id":"ayG7Wvn9wfqH"}}]}