{"nbformat":4,"nbformat_minor":0,"metadata":{"colab":{"provenance":[],"collapsed_sections":["bEkeDruCAxjX","BW08JjLCA-pk","mk0ca_LgCQ8b","-x6cl5W_OgDO"],"authorship_tag":"ABX9TyOUFVfFeL0E1PggvF4zef4O"},"kernelspec":{"name":"python3","display_name":"Python 3"},"language_info":{"name":"python"}},"cells":[{"cell_type":"markdown","source":["Summary of page 539 in Briggs is nice."],"metadata":{"id":"hwG5engf7ajZ"}},{"cell_type":"markdown","source":["### Question 1"],"metadata":{"id":"bEkeDruCAxjX"}},{"cell_type":"markdown","source":["(ex. 15, sec. 7.5, p. 540, Briggs) Evaluate\n","\n","$$\n","A = \\int \\frac{6}{x^2 - 1} \\, dx\n","$$"],"metadata":{"id":"Izh-pbjcAzSO"}},{"cell_type":"markdown","source":["#### Solution"],"metadata":{"id":"BW08JjLCA-pk"}},{"cell_type":"markdown","source":["\\begin{align}\n","\\frac{6}{x^2 - 1} &= \\frac{6}{(x+1)(x-1)} \\\\\n","&= \\frac{A}{x+1} + \\frac{B}{x-1} \\\\\n","6 &= (x-1)A + (x+1)B \\\\\n","0x + 6 &= x(A+B) + (B-A)\n","\\end{align}\n","It follows\n","\\begin{align}\n","0 &= A+B \\\\\n","6 &= B-A \\\\\n","A &= -3 \\\\\n","B &= 3\n","\\end{align}\n","So\n","\\begin{align}\n","A &= \\int \\frac{-3}{x+1} + \\frac{3}{x-1} \\\\\n","&= -3 \\int \\frac{1}{x+1} + 3 \\int \\frac{1}{x-1} \\\\\n","&= -3 \\ln |x+1| + 3 \\ln |x-1|\n","\\end{align}"],"metadata":{"id":"3kJSz2B3BBF7"}},{"cell_type":"markdown","source":["### Question 2"],"metadata":{"id":"mk0ca_LgCQ8b"}},{"cell_type":"markdown","source":["(ex. 30, sec. 7.5, p. 540, Briggs) Evaluate\n","\n","$$\n","A = \\int \\frac{1}{x^3 - 2x^2 - 4x + 8} \\, dx\n","$$"],"metadata":{"id":"6l3Yx7MKCTSy"}},{"cell_type":"markdown","source":["#### Solution"],"metadata":{"id":"q1wKYvedEbJC"}},{"cell_type":"markdown","source":["\\begin{align}\n","x^3 - 2x^2 - 4x + 8 &= x^3-4x - 2x^2 + 8 \\\\\n","&= x(x^2 - 4) - 2(x^2 - 4) \\\\\n","&= (x^2-4) (x-2) \\\\\n","&= (x+2) (x-2)^2\n","\\end{align}\n","\n","Then\n","\\begin{align}\n","\\frac{1}{x^3 - 2x^2 - 4x + 8} &= \\frac{1}{(x+2)(x-2)^2} = \\frac{A}{(x+2)} + \\frac{B}{(x-2)} + \\frac{C}{(x-2)^2} \\\\\n","1 &= (x-2)^2 A + (x+2)(x-2) B + (x+2) C \\\\\n","0x^2 + 0x + 1 &= (A + B)x^2 + (C-4A)x + (4A-4B+2C)\n","\\end{align}\n","\n","It follows\n","\\begin{align}\n","0 &= A+B \\\\\n","0 &= C-4A \\\\\n","1 &= 4A-4B+2C\n","\\end{align}\n","\n","In turn\n","\\begin{align}\n","B = -A \\\\\n","A = \\frac{C}{4}\n","\\end{align}\n","\n","Concluding\n","$$\n","1 = C + C + 2C = 4C\n","$$\n","\n","So\n","\\begin{align}\n","A &= \\frac{1}{16} \\\\\n","B &= \\frac{-1}{16} \\\\\n","C &= \\frac{1}{4}\n","\\end{align}\n","\n","Finally\n","\\begin{align}\n","A &= \\frac{1}{16} \\int \\frac{1}{x+2} + \\frac{-1}{16} \\int \\frac{1}{x-2} + \\frac{1}{4} \\int \\frac{1}{(x-2)^2} \\\\\n","&= \\frac{1}{16} \\ln |x+2| + \\frac{-1}{16} \\ln |x-2| + \\frac{-1}{4} \\frac{1}{x-2} + C\n","\\end{align}"],"metadata":{"id":"GwPFbNWUEcsW"}},{"cell_type":"markdown","source":["### Question 3"],"metadata":{"id":"-x6cl5W_OgDO"}},{"cell_type":"markdown","source":["(ex. 48, sec. 8.4, page. 541, Briggs) Evaluate\n","$$\n","A = \\int \\frac{2x + 1}{x^2 + 4} \\, dx\n","$$"],"metadata":{"id":"s6IW7mopOjqc"}},{"cell_type":"markdown","source":["#### Hints"],"metadata":{"id":"qw5kG1aL3nX6"}},{"cell_type":"markdown","source":["- You will use trigonometric substitution."],"metadata":{"id":"Sqy9VqWN3pYQ"}},{"cell_type":"markdown","source":["#### Solution"],"metadata":{"id":"r-3wF6R5OiXF"}},{"cell_type":"markdown","source":["$x^2 + 4$ is irreducible. Set\n","\n","\\begin{align}\n","\\frac{2x + 1 }{x^2 + 4} &= \\frac{Ax + B}{x^2 + 4} \\\\\n","2x + 1 &= Ax + B \\\\\n","2 &= A  \\\\\n","1 &= B\n","\\end{align}\n","It follows\n","\\begin{align}\n","A &= \\int \\frac{2x}{x^2+4} \\, dx + \\int \\frac{1}{x^2+4} \\, dx \\\\\n","&= \\int \\frac{du}{u} + \\int \\frac{1}{(2 \\tan \\theta)^2 + 2^2} \\, 2 \\sec^2 \\theta \\\\\n","&= \\ln |x^2 + 4| + \\int \\frac{1}{2^2 \\sec^2 \\theta} 2 \\sec^2 \\theta \\\\\n","&= \\ln |x^2 + 4| + \\frac{1}{2} \\int 1 \\, d\\theta \\\\\n","&= \\ln |x^2 + 4| + \\frac{1}{2} \\cdot \\theta \\\\\n","&= \\ln |x^2 + 4| + \\frac{1}{2} \\tan^{-1}(\\frac{x}{2})\n","\\end{align}"],"metadata":{"id":"9ONQ3UaLqmw4"}}]}