{"nbformat":4,"nbformat_minor":0,"metadata":{"colab":{"provenance":[],"collapsed_sections":["qHaP3V6oGYxM","oGmy6UHbHFLH","vk7UsHk9IEOA","RgniEep5p1Eh","BtHsvPyJqr9n","M9u5bfqFrHOL","tm9-5lAbwdDa","-M_dACGqxJHi"],"authorship_tag":"ABX9TyN/vzGUazkz4tlpiL11kf3k"},"kernelspec":{"name":"python3","display_name":"Python 3"},"language_info":{"name":"python"}},"cells":[{"cell_type":"markdown","source":["## On-Paper"],"metadata":{"id":"zW9TvksyGbAU"}},{"cell_type":"markdown","source":["### Question"],"metadata":{"id":"qHaP3V6oGYxM"}},{"cell_type":"markdown","source":["(ex. 23, p. 581, sec. 8.1, Briggs) Solve for $y$ given\n","\n","$$\n","y'(t) = 1 + e^t \\quad y(0) = 4\n","$$"],"metadata":{"id":"N7t8dbSCGgbO"}},{"cell_type":"markdown","source":["#### Solution"],"metadata":{"id":"oGmy6UHbHFLH"}},{"cell_type":"markdown","source":["\\begin{align}\n","y(t) &= \\int 1 + e^t = t + e^t + C \\\\\n","y(0) &= 0 + e^0 + C = 4 \\\\\n","&= 1 + C = 4 \\\\\n","C &= 3 \\\\\n","y(t) &= t + e^t + 3\n","\\end{align}"],"metadata":{"id":"er0HlkHoHL3q"}},{"cell_type":"markdown","source":["### Question"],"metadata":{"id":"vk7UsHk9IEOA"}},{"cell_type":"markdown","source":["(ex. 18, p. 595, sec. 8.3, Briggs) Solve the equation\n","\n","$$\n","\\sec t \\, y'(t) = 1, y(0) = 1\n","$$"],"metadata":{"id":"2vbRWqp5IM7-"}},{"cell_type":"markdown","source":["#### Solution"],"metadata":{"id":"RgniEep5p1Eh"}},{"cell_type":"markdown","source":["\\begin{align}\n","\\int y'(t) \\, dt &= \\int \\cos \\, dt \\\\\n","\\int dy &= \\sin t + c \\\\\n","y(t) &=  \\\\\n","y(0) &= \\sin 0 + c = 1 \\\\\n","&= c = 1 \\\\\n","y &= \\sin t + 1\n","\\end{align}"],"metadata":{"id":"5YNJcoFJp3uv"}},{"cell_type":"markdown","source":["### Question"],"metadata":{"id":"BtHsvPyJqr9n"}},{"cell_type":"markdown","source":["(ex. 24, p. 595, sec. 8.1, Briggs) Solve\n","\n","$$\n","\\sec x \\, y'(x) = y^3\n","$$"],"metadata":{"id":"hvQU5cvHquie"}},{"cell_type":"markdown","source":["#### Solution"],"metadata":{"id":"M9u5bfqFrHOL"}},{"cell_type":"markdown","source":["\\begin{align}\n","\\frac{1}{y^3} \\cdot y'(x) &= \\frac{1}{\\sec x} \\\\\n","\\int y^{-3} y' \\, dx &= \\int \\cos x \\, dx \\\\\n","\\int y^{-3} \\, dy &= \\sin x + c \\\\\n","\\frac{-1}{2} y^{-2} &= \\sin x + c \\\\\n","\\frac{-1}{2} \\cdot y^{-2} &= \\\\\n","\\frac{1}{y^2} &= -2 \\sin x + c\n","\\end{align}\n","\n","Since $y(0) = 3$\n","\n","\\begin{align}\n","\\frac{1}{3^2} &= -2 \\sin 0 + c \\\\\n","\\frac{1}{9} &= c\n","\\end{align}\n","\n","Therefore\n","\n","$$\n","\\frac{1}{y^2} = -2 \\sin x + \\frac{1}{9}\n","$$"],"metadata":{"id":"7ED149GmrJA4"}},{"cell_type":"markdown","source":["### Question"],"metadata":{"id":"tm9-5lAbwdDa"}},{"cell_type":"markdown","source":["(ex. 11, p. 603, sec. 8.4, Briggs) Solve the first-order differential equation\n","\n","$$\n","y'(t) = 3y - 6, y(0) = 9\n","$$"],"metadata":{"id":"xdkTOxYvwfxS"}},{"cell_type":"markdown","source":["#### Solution"],"metadata":{"id":"-M_dACGqxJHi"}},{"cell_type":"markdown","source":["\\begin{align}\n","b &= -6 \\\\\n","k &= 3 \\\\\n","y(t) &= C e^{3t} + \\frac{6}{3} \\\\\n","y(0) &= C + 2 = 9 \\\\\n","C &= 7 \\\\\n","y &= 7e^{3t} + 2\n","\\end{align}"],"metadata":{"id":"Vwup1oN1xLAu"}}]}