{"nbformat":4,"nbformat_minor":0,"metadata":{"colab":{"provenance":[],"collapsed_sections":["XcNmOMgep7_v","M1iFVYulj8Fb"],"authorship_tag":"ABX9TyPGO+6TFVBYp+RBmEAwN/UG"},"kernelspec":{"name":"python3","display_name":"Python 3"},"language_info":{"name":"python"}},"cells":[{"cell_type":"markdown","source":["### Question"],"metadata":{"id":"XcNmOMgep7_v"}},{"cell_type":"markdown","source":["(ex. 12 (a), p. 187, sec. 4.1, Kolman) Given\n","\n","$$\n","u = \\begin{bmatrix} 2 \\\\ 3 \\end{bmatrix}\n","\\quad\n","v = \\begin{bmatrix} -2 \\\\ 5 \\end{bmatrix}\n","$$\n","\n","Compute $u + v$, $u - v$, $2u$, and $3u-2v$."],"metadata":{"id":"OFjAxRXmkEeo"}},{"cell_type":"markdown","source":["#### Solution"],"metadata":{"id":"M1iFVYulj8Fb"}},{"cell_type":"markdown","source":["\\begin{align}\n","u + v &= \\begin{bmatrix} 2 + (-2) \\\\ 3 + 5 \\end{bmatrix} = \\begin{bmatrix} 0 \\\\ 8 \\end{bmatrix} \\\\\n","u - v &= \\begin{bmatrix} 2 - (-2) \\\\ 3 - 5 \\end{bmatrix} = \\begin{bmatrix} 4 \\\\ -2 \\end{bmatrix} \\\\\n","2u &= \\begin{bmatrix} 2 \\cdot 2 \\\\ 2 \\cdot 3 \\end{bmatrix} = \\begin{bmatrix} 4 \\\\ 6 \\end{bmatrix} \\\\\n","3u - 2v &= \\begin{bmatrix} 3 \\cdot 2 \\\\ 3 \\cdot 3 \\end{bmatrix} - \\begin{bmatrix} 2 \\cdot (-2) \\\\ 2 \\cdot 5 \\end{bmatrix} \\\\\n","&= \\begin{bmatrix} 6 \\\\ 9 \\end{bmatrix} - \\begin{bmatrix} -4 \\\\ 10 \\end{bmatrix} \\\\\n","&= \\begin{bmatrix} 6 - (-4) \\\\ 9 - 10 \\end{bmatrix} = \\begin{bmatrix} 10 \\\\ -1 \\end{bmatrix}\n","\\end{align}\n"],"metadata":{"id":"Ic3up2_vkyXP"}}]}